f(n) = a1 f(n-1) + a2 f(n-2) +... + am f(n-m) + g(n)
f(n) = X1 * b1 ^ n + X2 * b2 ^ n +... + Xm * bm ^ n + G(n)


     X1*b1 ^  n    + X2*b2 ^  n    + ... + Xm*bm ^  n    + G(n)    =  
a1 [ X1*b1 ^ (n-1) + X2*b2 ^ (n-1) + ... + Xm*bm ^ (n-1) + G(n-1)] +
a2 [ X1*b1 ^ (n-2) + X2*b2 ^ (n-2) + ... + Xm*bm ^ (n-2) + G(n-2)] +
a3 [ X1*b1 ^ (n-3) + X2*b2 ^ (n-3) + ... + Xm*bm ^ (n-3) + G(n-3)] +
... 								 ...					     ...
am [ X1*b1 ^ (n-m) + X2*b2 ^ (n-m) + ... + Xm*bm ^ (n-m) + G(n-m)] +
g(n)


b1 ^ n  = a1 * b1 ^ (n-1) + a2 * b1 ^ (n-2) + ... + am * b1 ^ (n-m)
b1 ^ m  = a1 * b1 ^ (m-1) + a2 * b1 ^ (m-2) + ... + am 
0 = (A1 - b1) (A2 - b1) (A3 - b1) ... (Am - b1)

G(n) = G(n-1) + G(n-2) + ... + G(n-m) + g(n)
G(n) - G(n-1) - G(n-2) - ... - G(n-m) = g(n)

======================================================================

a(n) = 3a(n−1)−2a(n−2)+2^n    a0 =4, a1 =9
n^2 =3n−2+2^n
n(n-3) =−2
n=1 n=2

a(n) = A*1^n + B*2^n + g(n)

C*2^n = 3/2*C*2^n - 2/4*C*2^n + 2^n
C*2^n - 3/2*C*2^n + 2/4*2^n = 2^n
C*2^n - 3/2*C*2^n + 2/4*2^n = 2^n


A*1^n + B*2^n + g(n)

a(n) = 3a(n−1)−2a(n−2)+2^n
A2^n = 3A/2*2^n*(n-1) - 2/4*A*2^n*(n-2) + 2^n
0 =  -3A/2*2^n + 4/4*A*2^n + 2^n
0 =  -3A/2 + 4/4*A + 1
0 =  -3/2*A + A + 1
0 =  -1/2*A + 1
A = 2

a(n) = A*1^n + B*2^n + 2*n*2^n
a(n) = A + B*2^n + 2*n*2^n
a(n) = A + B  =4
a(n) = A + B*2 + 2*2 =9
a(n) = A + B*2 =5
B =1
A=3

a(n) = 3 + 2^n + 2*n*2^n
a(n) = 3 + 2^n(1+2n)
an = (1 + 2n)2^n + 3

======================================================================


f(n) = 64 f(n-1)^2 / f(n-2)								a0 =8,a1 =1024
log2 f(n) = log2 64 + log2 f(n-1)^2 - log2 f(n-2)
log2 f(n) = 6 + 2*log2 f(n-1) - log2 f(n-2)
g(n) = log2 f(n)										g(0) =3,g(1) =10
g(n) = 6 + 2g(n-1) - g(n-2)
n^2 = 2n - 1
n(n-2) = -1
n=1 

n^2 A = 6 + 2A(n-1)^2 - A(n-2)^2
n^2 A = 6 + 2A(n^2-2n+1) - A(n^2-4n+4)
 = 6 - 2A
 A = 3


f(n) = (A+Bn)*1^n + 3*n^2
A  = 3
f(n) = (3+B) + 3 = 10
f(n) = 3+4*n + 3*n^2

f(2)=2046


======================================================================

f(n) = 2f(n-1) - f(n-2) + 16*5^n			f(0)=0 f(1)=101
x^2 = 2x - 1
x=1

A*5^n = A*2/5*5^n - A/25*5^n + 16*5^n
A*5^n*(1-2/5+1/25) = 16*5^n
A*(1-2/5+1/25) = 16
A*(25/25-10/25+1/25) = 16
A*(16/25) = 16
A/25 = 1
A=25


f(n) = (A+Bn)1^n + 25*5^n
f(0) = 0 = (A) + 25
f(1) = 101 = (A+B) + 25*5
A=-25
f(1) = 101 = (-25 + B) + 125
B=1
f(n) = n-25 + 25*5^n
f(n) = 2-25 + 25*5^2 = 602
f(2) = 2*101  + 16*5^2 = 602

